# AckerManFunction-For-4-0-4
Given an assessment to compute the ackerman function given:  
M = 4 
for n 0-4, 

We were also was given known shortcuts for the ackerman function, which were utilised to avoid recursion errors. 

Output: 
(2^( 1 + 3 ))- 3
Answer when m is 0 = (2^( 1 + 3 ))- 3
(2^( 1 + 3 ))- 3
2^((2^( 1 + 3 )))- 3
Answer when m is 1 = 2^((2^( 1 + 3 )))- 3
(2^( 1 + 3 ))- 3
2^((2^( 1 + 3 )))- 3
2^(2^((2^( 1 + 3 ))))- 3
Answer when m is 2 = 2^(2^((2^( 1 + 3 ))))- 3
(2^( 1 + 3 ))- 3
2^((2^( 1 + 3 )))- 3
2^(2^((2^( 1 + 3 ))))- 3
2^(2^(2^((2^( 1 + 3 )))))- 3
Answer when m is 3 = 2^(2^(2^((2^( 1 + 3 )))))- 3
(2^( 1 + 3 ))- 3
2^((2^( 1 + 3 )))- 3
2^(2^((2^( 1 + 3 ))))- 3
2^(2^(2^((2^( 1 + 3 )))))- 3
2^(2^(2^(2^((2^( 1 + 3 ))))))- 3
Answer when m is 4 = 2^(2^(2^(2^((2^( 1 + 3 ))))))- 3


